---
layout: page
title: Table of Derivatives
---



### Derivative Formulas

| $$\frac{d}{dx}x^n = nx^{n-1}$$                         | $$\frac{d}{dx}e^x = e^x$$                               |
| ------------------------------------------------------ | ------------------------------------------------------- |
| $$\frac{d}{dx}\sin x = \cos x$$                        | $$\frac{d}{dx}\cos x = -\sin x$$                        |
| $$\frac{d}{dx}\tan x = \sec^2 x$$                      | $$\frac{d}{dx}\cot x = -\csc^2 x$$                      |
| $$\frac{d}{dx}\sec x = \sec x \tan x $$                | $$\frac{d}{dx}\csc x = -\csc x \cot x $$                |
| $$\frac{d}{dx}\log x = \frac{1}{x}$$                   | $$\frac{d}{dx} a^x = \log(a) a^x$$                      |
| $$\frac{d}{dx}\arcsin x = \frac{1}{\sqrt{1-x^2}}$$     | $$\frac{d}{dx}\arccos x = -\frac{1}{\sqrt{1-x^2}}$$     |
| $$\frac{d}{dx}\arctan x = \frac{1}{1+x^2}$$            | $$\frac{d}{dx}\arccot x = -\frac{1}{1+x^2}$$            |
| $$\frac{d}{dx}\arcsec x = \frac{1}{\|x\|\sqrt{x^2-1}}$$  | $$\frac{d}{dx}\arccsc x = -\frac{1}{\|x\|\sqrt{x^2-1}}$$  |
| $$\frac{d}{dx}\sinh x = \cosh x$$                      | $$\frac{d}{dx}\cosh x = \sinh x$$                       |
| $$\frac{d}{dx}\tanh x = \sech^2 x $$                   | $$\frac{d}{dx}\coth x = -\csch^2 x$$                    |
| $$\frac{d}{dx}\sech x = \sech x \tanh x$$              | $$\frac{d}{dx}\csch x = -\csch x \coth x $$             |
| $$\frac{d}{dx}\arcsinh x = \frac{1}{\sqrt{x^2+1}}$$    | $$\frac{d}{dx}\arccosh x = \frac{1}{\sqrt{x^2-1}}$$     |
| $$\frac{d}{dx} \arctanh x = \frac{1}{1-x^2}$$          | $$\frac{d}{dx}\arccoth x = \frac{1}{1-x^2}$$            |
| $$\frac{d}{dx}\arcsech x = \frac{1}{\|x\|\sqrt{1-x^2}}$$ | $$\frac{d}{dx}\arccsch x = -\frac{1}{\|x\|\sqrt{1-x^2}}$$ |

### Differentiation Rules

$$\frac{d}{dx}\left[ f(x) + g(x) \right]  = \frac{df}{dx} + \frac{dg}{dx}$$

$$\frac{d}{dx}\left[\lambda f(x)\right] = \lambda \frac{df}{dx}$$

$$\frac{d}{dx}\left[f(x)g(x)\right] = \frac{df}{dx}g(x) + f(x)\frac{dg}{dx}$$

$$\frac{d}{dx}\left[\frac{f(x)}{g(x)}\right] = \frac{f'(x)g(x) - f(x)g'(x)}{g(x)^2}$$

$$\frac{d}{dx}f(g(x)) = \frac{df}{dg}\frac{dg}{dx}$$

