---
layout: lesson
title: The Bosonic Coherent State Path Integral - Exercises
dept: physics
course: many-body-II
unit: unit2
deptDisplay: Physics
courseDisplay: Many Body Physics II
unitDisplay: Unit 2
---
<ol>
\question In this problem, we will derive the expression for the coherent state for bosons. This state is an eigenstate of the boson annihilation operator, and so satisfies

$$\bhat\ket{z} = z\ket{z}.$$

It must also satisfy that \\(\bra{z}\ket{z} = 1\\). Using these two properties, derive an expression for the boson coherent state in terms of the basis \\(\ket{n}\\) signifying \\(n\\) particles in a particular state. 

\begin{solution}
As a first step, we will write
$$\ket{z} = \sum_{n=0}^\infty a_{nz}\ket{n}.$$
Our goal is to calculate \\(a_{nz}\\) such that \\(\ket{z}\\) satisfies the above two conditions. Our first step is to recast the two conditions into constraints on the coefficients \\(a_{nz}\\). Using the eigenstate condition, we find that 

$$\begin{align}
\bhat\ket{z} =& \bhat\sum_{n=0}^\infty a_{nz}\ket{n} \\
=& \sum_{n=0}^\infty a_{nz}\sqrt{n}\ket{n-1} \\
=& \sum_{n=1}^\infty a_{nz}\sqrt{n}\ket{n-1} \\
z\sum_{n=0}^\infty a_{nz}\ket{n} =& \sum_{n=0}^\infty a_{n+1,z}\sqrt{n+1}\ket{n}
\end{align}$$

and by matching coefficients, we find that 

$$za_{nz} = \sqrt{n+1}a_{n+1,z}$$

which gives us a recursion relation capturing the first constraint on our coefficients: 

$$\frac{a_{n+1,z}}{a_{nz}} = \frac{z}{\sqrt{n+1}}.$$

The second constraint of normalization simply yields that 

$$\sum_{n=0}^\infty |a_{nz}|^2 = 1.$$

Equipped with these constraints, we start by solving the recursion relation, which gives 

$$a_{nz} = \frac{z^n}{\sqrt{n!}}a_{0z}.$$

Now plugging this into the normalization condition, we find that 

$$\sum_{n=0}^\infty \frac{|z|^{2n}}{n!}|a_{0z}|^2 = 1 = e^{|z|^2}$$

and find that 

$$a_{0z} = e^{-|z|^2/2}.$$

Lastly, we write 

$$\begin{align}
\ket{z} =& e^{-|z|^2/2} \sum_{n=0}^\infty \frac{z^n}{\sqrt{n!}}\ket{n} \\
=& e^{-|z|^2/2}\sum_{n=0}^\infty \frac{z^n}{n!} \sqrt{n!}\ket{n} \\
=& e^{-|z|^2/2}\sum_{n=0}^\infty \frac{z^n}{n!} (\bhat^\dagger)^n \ket{0} \\
=& e^{-|z|^2/2} e^{z\bhat^\dagger}\ket{0}
\end{align}$$

\end{solution}

\end{questions}

