---
layout: lesson
title: The Euler Lagrange Equation
dept: physics
course: cm-III
unit: unit1
deptDisplay: Physics
courseDisplay: Classical Mechanics III
unitDisplay: Unit 1
---

In this lesson, we will derive the Euler-Lagrange equation for the basic problem in the calculus of variations. The problem is to minimize the integral

$$S[x] = \int_a^b \mathcal{L}(t,x,\dot{x}) dt $$

over differentiable functions $x$, where $x(a)$ and $x(b)$ are given. To do this, we assume that we have found a function $x_{\*}$ which minimizes the integral. Then, we consider a general function $x = x_{\*} + \epsilon\eta$, where $\eta$ is a any function satisfying $\eta(a) = \eta(b) = 0$; recall that we are only considering functions which satisfy the boundary conditions so we cannot have any extra contributions at $t = a$ and $t = b$. Thus, $\epsilon\eta$ is a small perturbing funciton. We note that for $\epsilon = 0$, $y$ becomes the minimizer of the integral. This means that 

$$\frac{d}{d\epsilon} S[x]\bigg|_{\epsilon = 0} = 0.$$

Armed with this condition, we compute the derivative of $S$ with respect to $\epsilon$. 

$$\begin{eqnarray*}
\frac{d}{d\epsilon}S[x] &=& \frac{d}{d\epsilon} \int_a^b \mathcal{L}(t,x,\dot{x}) dt\\
&=& \int_a^b\left(\frac{\partial\mathcal{L}}{\partial x}\frac{dx}{d\epsilon} + \frac{\partial\mathcal{L}}{\partial \dot{x}} \frac{d\dot{x}}{d\epsilon}\right) dt \\
&=& \int_a^b\left(\frac{\partial\mathcal{L}}{\partial x}\eta + \frac{\partial\mathcal{L}}{\partial \dot{x}} \dot{\eta} \right) dt \\
&=&  \int_a^b\left(\frac{\partial\mathcal{L}}{\partial x}\eta \right) dt +  \int_a^b\left(\frac{\partial\mathcal{L}}{\partial \dot{x}} \dot{\eta} \right) dt \\
&=&  \int_a^b\left(\frac{\partial\mathcal{L}}{\partial x}\eta \right) dt +  \left(\frac{\partial\mathcal{L}}{\partial \dot{x}} \eta\right)\bigg|_a^b - \int_a^b \frac{d}{dt}\left(\frac{\partial\mathcal{L}}{\partial \dot{x}} \right)\eta dt \\
&=&  \int_a^b\left[\frac{\partial\mathcal{L}}{\partial x}- \frac{d}{dt}\left(\frac{\partial\mathcal{L}}{\partial \dot{x}} \right)\right]\eta dt 
\\
&=& 0
\end{eqnarray*}$$

Since this integral is 0 for all $\eta$, we conclude that the object multiplying it is zero, or, 

$$\frac{\partial\mathcal{L}}{\partial x}- \frac{d}{dt}\left(\frac{\partial\mathcal{L}}{\partial \dot{x}}\right)  = 0$$

This is known as the Euler-Lagrange equation. 

<div class="result">
<b>Result:</b> If the function $x(t)$ is a stationary point of the functional 
$$S[x] = \int_a^b \mathcal{L}(t,x,\dot{x}) dt,$$
then it must satisfy the <i>Euler Lagrange equation</i>
$$\frac{\partial\mathcal{L}}{\partial x}- \frac{d}{dt}\left(\frac{\partial\mathcal{L}}{\partial \dot{x}}\right)  = 0.$$
</div>

<br> 

Note that in this derivation, we have $t$ as the independent variable and $x = x(t)$ as the dependent variable. The Euler Lagrange equation works equally well if we simply relabel the variables; some problems have $x$ as the independent variable and $y = y(x)$ as the dependent variable. In these cases we have $\L = \L(x,y,y')$ and the Euler Lagrange equation is 

$$\frac{\partial\L}{\partial y} = \frac{d}{dx}\frac{\partial\L}{\partial y'}.$$

### Examples
To get a feel for how this works, let us now find the Euler Lagrange equation for certain Lagrangians. 

<div class="example">
<p><b>Example:</b> Find the Euler Lagrange equation for the Lagrangian
$$\L(x,\dot{x}) = \frac{1}{2}m\dot{x}^2 - V(x),$$
where $m$ is a constant. Does the resulting equation look familiar? </p>
<b>Solution:</b> 
</div>

<br>

<div class="example">
<p><b>Example:</b> 
<ol type = "a">
<li> Find the Euler Lagrange equation for the Lagrangian corresponding to the shortest path between two points:
$$\L(y,y') = \sqrt{1+(y')^2}$$
</li>
<li> Solve the differential equation subject to boundary conditions $y(x_1) = y_1$ and $y(x_2) = y_2$. </li> 
</ol> </p>
<b>Solution:</b>
<ol type = "a">
<li> </li>
<li> </li>
</ol>
</div>

<br>

<div class="example">
<p><b>Example:</b> Find the Euler Lagrange equation for the Lagrangian 
$$\L(y,y') = y\sqrt{1+(y')^2},$$
which you may recognize as the one from the minimal lateral surface area problem from the introduction page. You do not need to solve the resulting differential equation. </p>
<b>Solution:</b> The Euler Lagrange equation for us is (consider $x$ the independent variable and $y$ the dependent variable)
$$\frac{d}{dx}\left(\frac{\partial\mathcal{L}}{\partial y'}\right) = \frac{\partial\mathcal{L}}{\partial y}.$$

If we plug this in, we find that the partial derivatives of $\L$ with respect to $y$ and $y'$ are, respectively,

$$\frac{\partial \L}{\partial y} = \sqrt{1+(y')^2} ,\qquad \frac{\partial\L}{\partial y'} = \frac{yy'}{\sqrt{1+(y')^2}}.$$

If we plug these into the Euler Lagrange equation, we get 

$$ \frac{d}{dx}\left(\frac{yy'}{\sqrt{1+(y')^2}}\right) = \sqrt{1+(y')^2}.$$

If we expand out all the terms, then we get 

$$\frac{(y')^2}{\sqrt{1+(y')^2}} +  \frac{yy''}{\sqrt{1+(y')^2}} - \frac{y(y')^2y''}{(1+(y')^2)^{3/2}}= \sqrt{1+(y')^2}$$

If we simplify the terms and cancel, then we get 

$$\frac{yy''}{1+(y')^2} = 1.$$

If we solve this differential equation for $y$, then we will find a function which provides a stationary point of the integral and thus minimizes the surface area.
</div>



